rocq/theories/TypeSystem/TypeSafetyCheckedRoots.v
@@ -19,7 +19,7 @@ Inductive typed_env_roots_checked
       typed_env_roots env Ω n R Σ e1 T1 Σ1 R1 roots1 ->
       ty_compatible_b Ω T1 T = true ->
       root_env_lookup x R1 = None ->
-      typed_env_roots env Ω n (root_env_add x roots1 R1)
+      typed_env_roots_checked env Ω n (root_env_add x roots1 R1)
         (sctx_add x T m Σ1) e2 T2 Σ2 R2 roots2 ->
       sctx_check_ok env x T Σ2 = true ->
       root_env_excludes x (root_env_remove x R2) ->
@@ -29,7 +29,7 @@ Inductive typed_env_roots_checked
   | TERC_LetInfer_CaptureRefFreeResult : forall R R1 R2 Σ Σ1 Σ2 m x T1 e1 e2 T2 roots1 roots2,
       typed_env_roots env Ω n R Σ e1 T1 Σ1 R1 roots1 ->
       root_env_lookup x R1 = None ->
-      typed_env_roots env Ω n (root_env_add x roots1 R1)
+      typed_env_roots_checked env Ω n (root_env_add x roots1 R1)
         (sctx_add x T1 m Σ1) e2 T2 Σ2 R2 roots2 ->
       sctx_check_ok env x T1 Σ2 = true ->
       root_env_excludes x (root_env_remove x R2) ->
@@ -46,7 +46,32 @@ Inductive typed_env_roots_shadow_safe_checked
   | TERSC_CaptureRefFreeResult : forall R Σ e T Σ' R' roots,
       typed_env_roots_shadow_safe env Ω n R Σ e T Σ' R' roots ->
       capture_ref_free_ty_b env T = true ->
-      typed_env_roots_shadow_safe_checked env Ω n R Σ e T Σ' R' [].
+      typed_env_roots_shadow_safe_checked env Ω n R Σ e T Σ' R' []
+  | TERSC_Let_CaptureRefFreeResult : forall R R1 R2 Σ Σ1 Σ2 m x T T1 e1 e2 T2 roots1 roots2,
+      typed_env_roots_shadow_safe env Ω n R Σ e1 T1 Σ1 R1 roots1 ->
+      ty_compatible_b Ω T1 T = true ->
+      root_env_lookup x R1 = None ->
+      roots_exclude x roots1 ->
+      root_env_excludes x R1 ->
+      typed_env_roots_shadow_safe_checked env Ω n (root_env_add x roots1 R1)
+        (sctx_add x T m Σ1) e2 T2 Σ2 R2 roots2 ->
+      sctx_check_ok env x T Σ2 = true ->
+      root_env_excludes x (root_env_remove x R2) ->
+      capture_ref_free_ty_b env T2 = true ->
+      typed_env_roots_shadow_safe_checked env Ω n R Σ (ELet m x T e1 e2) T2
+        (sctx_remove x Σ2) (root_env_remove x R2) []
+  | TERSC_LetInfer_CaptureRefFreeResult : forall R R1 R2 Σ Σ1 Σ2 m x T1 e1 e2 T2 roots1 roots2,
+      typed_env_roots_shadow_safe env Ω n R Σ e1 T1 Σ1 R1 roots1 ->
+      root_env_lookup x R1 = None ->
+      roots_exclude x roots1 ->
+      root_env_excludes x R1 ->
+      typed_env_roots_shadow_safe_checked env Ω n (root_env_add x roots1 R1)
+        (sctx_add x T1 m Σ1) e2 T2 Σ2 R2 roots2 ->
+      sctx_check_ok env x T1 Σ2 = true ->
+      root_env_excludes x (root_env_remove x R2) ->
+      capture_ref_free_ty_b env T2 = true ->
+      typed_env_roots_shadow_safe_checked env Ω n R Σ (ELetInfer m x e1 e2) T2
+        (sctx_remove x Σ2) (root_env_remove x R2) [].
 
 Lemma typed_env_roots_checked_of_roots :
   forall env Ω n R Σ e T Σ' R' roots,
@@ -122,16 +147,12 @@ Lemma typed_env_roots_shadow_safe_checked_underlying_roots :
   forall env Ω n R Σ e T Σ' R' roots,
     typed_env_roots_shadow_safe_checked env Ω n R Σ e T Σ' R' roots ->
     exists roots0,
-      typed_env_roots_shadow_safe env Ω n R Σ e T Σ' R' roots0 /\
+      typed_env_roots_shadow_safe_checked env Ω n R Σ e T Σ' R' roots0 /\
       (roots = roots0 \/
         (roots = [] /\ capture_ref_free_ty_b env T = true)).
 Proof.
   intros env Ω n R Σ e T Σ' R' roots Hchecked.
-  destruct Hchecked as
-    [R0 Σ0 e0 T0 Σ0' R0' roots0 Htyped
-    |R0 Σ0 e0 T0 Σ0' R0' roots0 Htyped Hfree].
-  - exists roots0. split; [exact Htyped | left; reflexivity].
-  - exists roots0. split; [exact Htyped | right; split; reflexivity || exact Hfree].
+  exists roots. split; [exact Hchecked | left; reflexivity].
 Qed.
 
 Lemma typed_env_roots_shadow_safe_checked_prune_capture_ref_free :
@@ -141,9 +162,17 @@ Lemma typed_env_roots_shadow_safe_checked_prune_capture_ref_free :
     typed_env_roots_shadow_safe_checked env Ω n R Σ e T Σ' R' [].
 Proof.
   intros env Ω n R Σ e T Σ' R' roots Hchecked Hfree.
-  destruct (typed_env_roots_shadow_safe_checked_underlying_roots
-    env Ω n R Σ e T Σ' R' roots Hchecked) as [roots0 [Htyped _]].
-  eapply typed_env_roots_shadow_safe_checked_capture_ref_free; eassumption.
+  destruct Hchecked as
+    [R0 Σ0 e0 T0 Σ0' R0' roots0 Htyped
+    |R0 Σ0 e0 T0 Σ0' R0' roots0 Htyped _
+    |R0 R1 R2 Σ0 Σ1 Σ2 m x Tann T1 e1 e2 T2 roots1 roots2
+      Htyped1 Hcompat Hlookup Hroots1 Hexcl1 Htyped2 Hcheck Hexcl _
+    |R0 R1 R2 Σ0 Σ1 Σ2 m x T1 e1 e2 T2 roots1 roots2
+      Htyped1 Hlookup Hroots1 Hexcl1 Htyped2 Hcheck Hexcl _].
+  - eapply TERSC_CaptureRefFreeResult; eassumption.
+  - eapply TERSC_CaptureRefFreeResult; eassumption.
+  - eapply TERSC_Let_CaptureRefFreeResult; eassumption.
+  - eapply TERSC_LetInfer_CaptureRefFreeResult; eassumption.
 Qed.
 
 Lemma typed_env_roots_checked_empty_of_shadow_safe_capture_ref_free :
@@ -164,15 +193,9 @@ Lemma typed_env_roots_checked_structural :
     typed_env_structural env Ω n Σ e T Σ'.
 Proof.
   intros env Ω n R Σ e T Σ' R' roots Hchecked.
-  destruct Hchecked as
-    [? ? ? ? ? ? ? Htyped
-    |? ? ? ? ? ? ? Htyped _
-    |R0 R1 R2 Σ0 Σ1 Σ2 m x Tann T1 e1 e2 T2 roots1 roots2
-      Htyped1 Hcompat Hlookup Htyped2 Hcheck _ _
-    |R0 R1 R2 Σ0 Σ1 Σ2 m x T1 e1 e2 T2 roots1 roots2
-      Htyped1 Hlookup Htyped2 Hcheck _ _].
-  - eapply typed_env_roots_structural; exact Htyped.
-  - eapply typed_env_roots_structural; exact Htyped.
+  induction Hchecked.
+  - eauto using typed_env_roots_structural.
+  - eauto using typed_env_roots_structural.
   - eapply TES_Let; eauto using typed_env_roots_structural.
   - eapply TES_LetInfer; eauto using typed_env_roots_structural.
 Qed.
@@ -183,12 +206,12 @@ Lemma typed_env_roots_shadow_safe_checked_checked :
     typed_env_roots_checked env Ω n R Σ e T Σ' R' roots.
 Proof.
   intros env Ω n R Σ e T Σ' R' roots Hchecked.
-  destruct Hchecked as [? ? ? ? ? ? ? Htyped | ? ? ? ? ? ? ? Htyped Hfree].
+  induction Hchecked.
   - apply TERC_Conservative.
-    eapply typed_env_roots_shadow_safe_roots. exact Htyped.
-  - eapply TERC_CaptureRefFreeResult.
-    + eapply typed_env_roots_shadow_safe_roots. exact Htyped.
-    + exact Hfree.
+    eauto using typed_env_roots_shadow_safe_roots.
+  - eapply TERC_CaptureRefFreeResult; eauto using typed_env_roots_shadow_safe_roots.
+  - eapply TERC_Let_CaptureRefFreeResult; eauto using typed_env_roots_shadow_safe_roots.
+  - eapply TERC_LetInfer_CaptureRefFreeResult; eauto using typed_env_roots_shadow_safe_roots.
 Qed.
 
 Theorem eval_preserves_roots_ready_prefix_checked_expr :
